



TRANSPROSE OF KERNEL

13

$$\langle Kf, g \rangle_\pi = \int_{\mathbb{X}} Kf(x)g(x)\pi(\mathrm{d}x)$$



Proof: Using the definition we compute both sides:

$$\langle f, K^\top g \rangle_\pi = \int_{\mathcal{X}} f(x') K^\top g(x') \pi(\mathrm{d}x')$$

- Given an π -invariant kernel, K in $L^2(\pi)$ we define the adjoint (or transpose) as K^\top if all $f, g \in L^2(\pi)$ we have

$$\langle Kf, g \rangle_\pi = \langle f, K^\top g \rangle_\pi$$

▶ We see they are equivalent if and only if detailed balance holds

► **Proposition:** The adjoint kernel satisfies

$$\pi(\mathrm{d}x)K(x, \mathrm{d}x') = \pi(\mathrm{d}x')K^\top(x', \mathrm{d}x)$$

► K is π -reversible if and only if K is self-adjoint $K \equiv K^T$

$$= \int_X \int_X K(x, dx') f(x') g(x) \pi(dx)$$

$$= \int_{\mathcal{X}} \int_{\mathcal{X}} f(x') K^{\top}(x', \mathrm{d}x) g(x) \pi(\mathrm{d}x')$$

TRANSPOSE OF KERNEL

13

- ▶ Given an π -invariant kernel, K in $L^2(\pi)$ we define the adjoint (or transpose) as K^\top if all $f, g \in L^2(\pi)$ we have

$$\langle Kf, g \rangle_\pi = \langle f, K^\top g \rangle_\pi$$

- ▶ **Proposition:** The adjoint kernel satisfies

$$\pi(\mathrm{d}x)K(x, \mathrm{d}x') = \pi(\mathrm{d}x')K^\top(x', \mathrm{d}x)$$

- ▶ K is π -reversible if and only if K is self-adjoint $K = K^\top$
- ▶ **Proof:** Using the definition we compute both sides:
$$\begin{aligned}\langle Kf, g \rangle_\pi &= \int_{\mathbb{X}} Kf(x)g(x)\pi(\mathrm{d}x) = \int_{\mathbb{X}} \int_{\mathbb{X}} K(x, \mathrm{d}x')f(x')g(x)\pi(\mathrm{d}x) \\ \langle f, K^\top g \rangle_\pi &= \int_{\mathbb{X}} f(x')K^\top g(x')\pi(\mathrm{d}x') = \int_{\mathbb{X}} \int_{\mathbb{X}} f(x')K^\top(x', \mathrm{d}x)g(x)\pi(\mathrm{d}x')\end{aligned}$$
- ▶ We see they are equivalent if and only if detailed balance holds

ALGEBRA OF KERNELS